src/tlogic/SimWeakest.v
@@ -1433,3 +1433,5 @@ From Fairness Require Export LinkingRed.
 
 Ltac lred2 := (prw ltac:(red_tac itree_class) 1 2 0).
 Ltac rred2 := (prw ltac:(red_tac itree_class) 1 1 0).
+Ltac lred2r := repeat lred2.
+Ltac rred2r := repeat rred2.
